compose/Sem.v
@@ -27,24 +27,16 @@ Local Open Scope asm.
 
 Module Frame.
 
-  (* Naming Candidates *)
-  (* Module -> Short pronunciation. its shorhand "m" conflicts with "m" of "memory". *)
-  (* StackFrame (Activation Record) -> Too long *)
-  (* Frame -> Short, also it is quite clear (Frame is not used elsewhere in this level) *)
-
   Record t: Type := mk {
     ms: ModSem.t;
-    rs_init: regset;
+    (* st_init: ms.(ModSem.state); *)
     st: ms.(ModSem.state); (* local state *)
   }
   .
 
   Definition update_st (fr0: t) (st0: fr0.(ms).(ModSem.state)): t :=
-    (mk fr0.(ms) fr0.(rs_init) st0)
+    (mk fr0.(ms) st0)
   .
-
-(* Definition is_internal (fr0: t): Prop := fr0.(ms).(ModSem.is_internal) fr0.(st) fr0.(sg_arg) fr0.(rs_arg). *)
-  (* Definition is_internal (fr0: t): Prop := fr0.(ms).(ModSem.is_internal) fr0.(st). *)
 
 End Frame.
 
@@ -52,25 +44,7 @@ End Frame.
 
 Module Ge.
 
-  (* NAMING: Consistency with SkEnv.t -> GEnv.t? but this is confusing with Genv *)
-  (* Record t: Type := mk { *)
-  (*   mss: list ModSem.t; *)
-  (* } *)
-  (* . *)
-
   Definition t: Type := list ModSem.t.
-
-  (* Note: nat is much more convenient in SimLoad. (find_fptr_owner bsim) && stating disjointness. *)
-  (* If needed, fefactor later to hide these details *)
-
-  (* Inductive find_fptr_owner (ge: t) (fptr: val) (ms: ModSem.t): Prop := *)
-  (* | find_fptr_owner_intro *)
-  (*     blk *)
-  (*     (FPTR: fptr = Vptr blk Ptrofs.zero true) *)
-  (*     (MODSEM: In ms ge) *)
-  (*     if_sig *)
-  (*     (INTERNAL: Genv.find_def ms.(ModSem.skenv) blk = Some (Gfun (Internal if_sig))) *)
-  (* . *)
 
   Inductive find_fptr_owner (ge: t) (fptr: val) (ms: ModSem.t): Prop :=
   | find_fptr_owner_intro
@@ -78,19 +52,6 @@ Module Ge.
       if_sig
       (INTERNAL: Genv.find_funct ms.(ModSem.skenv) fptr = Some (Internal if_sig))
   .
-
-  (* Inductive find_fptr_owner (ge: t) (fptr: val) (n: nat): Prop := *)
-  (* | find_fptr_owner_intro *)
-  (*     blk *)
-  (*     (FPTR: fptr = Vptr blk Ptrofs.zero true) *)
-  (*     ms *)
-  (*     (MODSEM: List.nth_error ge n = Some ms) *)
-  (*     if_sig *)
-  (*     (INTERNAL: Genv.find_def ms.(ModSem.skenv) blk = Some (Gfun (Internal if_sig))) *)
-  (* . *)
-
-  (* Definition no_fptr_owner (ge: t) (fptr: val): Prop := *)
-  (*   List.Forall (not <*> find_fptr_owner ge fptr) ge. *)
 
   Inductive disjoint (ge: t): Prop :=
   | disjoint_intro
@@ -106,44 +67,28 @@ End Ge.
 
 Inductive state: Type :=
 | Callstate
-    (rs: regset)
-    (m: mem)
+    (args: Args.t)
     (frs: list Frame.t)
 | State
     (frs: list Frame.t)
 .
 
-(* If both are some, they are equal. *)
-Definition compat_sig (sg0: option signature) (sg1: option signature): bool :=
-  match sg0 with
-  | None => true
-  | Some sg0 => match sg1 with
-           | None => true
-           | Some sg1 => signature_eq sg0 sg1
-           end
-  end
-.
-
-(* Naming -> fr0/fr1 instead of fr_fst fr_snd. There will not be many fr_fst simultaneously, so it is OK *)
 Inductive step (ge: Ge.t): state -> trace -> state -> Prop :=
 | step_call
-    fr0 frs
-    rs_arg m_arg
-    (AT: fr0.(Frame.ms).(ModSem.at_external) fr0.(Frame.st) rs_arg m_arg)
+    fr0 frs args
+    (AT: fr0.(Frame.ms).(ModSem.at_external) fr0.(Frame.st) args)
   :
     step ge (State (fr0 :: frs))
-         E0 (Callstate rs_arg m_arg (fr0 :: frs))
+         E0 (Callstate args (fr0 :: frs))
 
 | step_init
-    rs_arg m_arg frs
-    fptr_arg ms
-    (FPTR: fptr_arg = rs_arg PC)
-    (MSFIND: ge.(Ge.find_fptr_owner) fptr_arg ms)
+    args frs ms
+    (MSFIND: ge.(Ge.find_fptr_owner) args.(Args.fptr) ms)
     st_init
-    (INIT: ms.(ModSem.initial_frame) rs_arg m_arg st_init)
+    (INIT: ms.(ModSem.initial_frame) args st_init)
   :
-    step ge (Callstate rs_arg m_arg frs)
-         E0 (State ((Frame.mk ms rs_arg st_init) :: frs))
+    step ge (Callstate args frs)
+         E0 (State ((Frame.mk ms st_init) :: frs))
 
 | step_internal
     fr0 frs
@@ -155,11 +100,10 @@ Inductive step (ge: Ge.t): state -> trace -> state -> Prop :=
          tr (State ((fr0.(Frame.update_st) st0) :: frs))
 | step_return
     fr0 fr1 frs
-    rs_ret
-    (FINAL: fr0.(Frame.ms).(ModSem.final_frame) fr0.(Frame.rs_init) fr0.(Frame.st) rs_ret)
+    retv
+    (FINAL: fr0.(Frame.ms).(ModSem.final_frame) fr0.(Frame.st) retv)
     st0
-    (AFTER: fr1.(Frame.ms).(ModSem.after_external) fr1.(Frame.st) fr0.(Frame.rs_init) rs_ret
-                                                   fr0.(Frame.st).(ModSem.get_mem fr0.(Frame.ms)) st0)
+    (AFTER: fr1.(Frame.ms).(ModSem.after_external) fr1.(Frame.st) retv st0)
   :
     step ge (State (fr0 :: fr1 :: frs))
          E0 (State ((fr1.(Frame.update_st) st0) :: frs))
@@ -179,45 +123,57 @@ Section SEMANTICS.
   (* Definition init_skenv: option SkEnv.t := option_map (@Genv.globalenv (fundef unit) unit) init_sk. *)
   (* Definition init_skenv (init_sk: Sk.t): SkEnv.t := (@Genv.globalenv (fundef (option signature)) unit) init_sk. *)
 
-  Definition load_modsems (skenv: SkEnv.t): list ModSem.t :=
-    (System.modsem skenv) :: List.map ((flip Mod.modsem) skenv) p.
+  Definition skenv_fill_internals (skenv: SkEnv.t): SkEnv.t :=
+    skenv.(Genv_map_defs) (fun _ gd =>
+                             Some
+                               match gd with
+                               | Gfun (External ef) => (Gfun (Internal ef.(ef_sig)))
+                               | Gfun _ => gd
+                               | Gvar gv => gd
+                               end)
+  .
+
+  Definition load_system (skenv: SkEnv.t): (ModSem.t * SkEnv.t) :=
+    (System.modsem skenv, skenv.(skenv_fill_internals))
+  .
+
+  Definition load_modsems (skenv: SkEnv.t): list ModSem.t := List.map ((flip Mod.modsem) skenv) p.
 
   (* Definition init_mem: option mem := option_join (option_map (@Genv.init_mem (fundef unit) unit) init_sk). *)
   (* Definition init_mem (init_sk: Sk.t): option mem := (@Genv.init_mem (fundef (option signature)) unit) init_sk. *)
 
   (* Definition init_genv: option Ge.t := *)
   (*   option_map (fun skenv => (Ge.mk skenv (init_modsem skenv))) init_skenv. *)
-  Definition load_genv (init_skenv: SkEnv.t): Ge.t := (load_modsems init_skenv).
+  Definition load_genv (init_skenv: SkEnv.t): Ge.t :=
+    let (system, skenv) := load_system init_skenv in
+    system :: (load_modsems skenv)
+  .
 
   (* Making dummy_module that calls main? => Then what is sk of it? Memory will be different with physical linking *)
   Inductive initial_state: state -> Prop :=
   | initial_state_intro
-      sk_link skenv_link m_init ge
+      sk_link skenv_link m_init
       (INITSK: link_sk = Some sk_link)
       (INITSKENV: sk_link.(Sk.load_skenv) = skenv_link)
       (INITMEM: sk_link.(Sk.load_mem) = Some m_init)
-      (INITGENV: load_genv (skenv_link) = ge)
-
-      rs_init
-      (INITREG: rs_init = init_regs (Genv.symbol_address skenv_link sk_link.(prog_main) Ptrofs.zero))
+      fptr_init
+      (FPTR: fptr_init = (Genv.symbol_address skenv_link sk_link.(prog_main) Ptrofs.zero))
+      (SIG: skenv_link.(Genv.find_funct) fptr_init = Some (Internal signature_main))
     :
-      initial_state (Callstate rs_init m_init [])
+      initial_state (Callstate (Args.mk fptr_init [] m_init) [])
   .
 
   Inductive final_state: state -> int -> Prop :=
   | final_state_intro
-      fr0
-      rs_ret
-      (FINAL: fr0.(Frame.ms).(ModSem.final_frame) fr0.(Frame.rs_init) fr0.(Frame.st)
-                                                    rs_ret)
-      reti
-      (RETPC: rs_ret#PC = Vnullptr)
-      (RETV: rs_ret#RAX = Vint reti)
+      fr0 retv
+      (FINAL: fr0.(Frame.ms).(ModSem.final_frame) fr0.(Frame.st) retv)
+      i
+      (INT: retv.(Retv.v) = Vint i)
     :
-      final_state (State [fr0]) reti
+      final_state (State [fr0]) i
   .
 
-  Definition semantics: semantics :=
+  Definition sem: semantics :=
     (Semantics_gen step initial_state final_state
                    (match link_sk with
                     | Some sk_link => load_genv sk_link.(Sk.load_skenv)
