compose/System.v
@@ -18,90 +18,72 @@ Section SYSMODSEM.
 
   Variable skenv_link: SkEnv.t.
 
-  Definition genvtype: Type := Genv.t (AST.fundef external_function) unit.
+  Definition genvtype: Type := Genv.t external_function unit.
 
   Definition globalenv: genvtype :=
     skenv_link.(Genv_map_defs) (fun _ gd =>
                                   match gd with
-                                  | Gfun (External ef) => Some (Gfun (Internal ef))
+                                  | Gfun (External ef) => Some (Gfun ef)
                                   | Gfun _ => None
                                   | Gvar gv => Some (Gvar gv)
                                   end)
   .
 
-  Definition skd: Type := globdef (fundef (option signature)) unit.
+  Definition skd: Type := globdef (fundef signature) unit.
 
-  Definition gd_to_skd V (gd: globdef (AST.fundef external_function) V): option skd :=
+  Definition gd_to_skd V (gd: globdef external_function V): skd :=
     match gd with
-    | Gfun (Internal ef) => Some (Gfun (Internal (Some ef.(ef_sig))))
-    | Gfun (External _) => None (* This should not happen *)
-    | Gvar (mkglobvar info init ro volatile) => Some (Gvar (mkglobvar tt init ro volatile))
+    | Gfun ef => (Gfun (Internal ef.(ef_sig)))
+    | Gvar (mkglobvar info init ro volatile) => (Gvar (mkglobvar tt init ro volatile))
     end
   .
 
   Definition skenv: SkEnv.t :=
-    globalenv.(Genv_map_defs) (fun _ gd => gd.(gd_to_skd))
+    globalenv.(Genv_map_defs) (fun _ gd => Some gd.(gd_to_skd))
   .
 
   Inductive state: Type :=
-  | state_call
-      (rs_arg: regset)
-      (m_arg: mem)
-  | state_return
-      (rs_ret: regset)
-      (m_ret: mem)
+  | Callstate
+      (args: Args.t)
+  | Returnstate
+      (retv: Retv.t)
   .
 
   Inductive step (ge: genvtype): state -> trace -> state -> Prop :=
   | step_intro
-      rs_arg m_arg ef
-      (FPTR: ge.(Genv.find_funct) (rs_arg PC) = Some (Internal ef))
-      vs
-      (ARGS: extcall_arguments rs_arg m_arg ef.(ef_sig) vs)
-      tr v_ret m_ret
-      (EXTCALL: external_call ef ge vs m_arg tr v_ret m_ret)
-      rs_ret
-      (RET: rs_ret = (set_pair (loc_external_result (ef_sig ef)) v_ret
-                               (undef_regs (List.map preg_of destroyed_at_call) rs_arg)))
+      args ef
+      (FPTR: ge.(Genv.find_funct) args.(Args.fptr) = Some ef)
+      tr retv
+      (EXTCALL: external_call ef ge args.(Args.vs) args.(Args.m) tr retv.(Retv.v) retv.(Retv.m))
     :
-      step ge (state_call rs_arg m_arg) tr (state_return rs_ret m_ret)
+      step ge (Callstate args) tr (Returnstate retv)
   .
 
-  Definition get_mem (st0: state): mem :=
-    match st0 with
-    | state_call _ m => m
-    | state_return _ m => m
-    end
-  .
-
-  Inductive initial_frame (rs_arg: regset) (m_arg: mem):
-    state -> Prop :=
+  Inductive initial_frame (args: Args.t): state -> Prop :=
   | initial_frame_intro
     :
-      initial_frame rs_arg m_arg (state_call rs_arg m_arg)
+      initial_frame args (Callstate args)
   .
 
-  Inductive final_frame (rs_init: regset): state -> regset -> Prop :=
+  Inductive final_frame: state -> Retv.t -> Prop :=
   | final_frame_intro
-      rs_ret m_ret
+      retv
     :
-      final_frame rs_init (state_return rs_ret m_ret) rs_ret
+      final_frame (Returnstate retv) retv
   .
 
   Program Definition modsem: ModSem.t := {|
     ModSem.state := state;
     ModSem.genvtype := genvtype;
     ModSem.step := step;
-    ModSem.get_mem := get_mem;
-    ModSem.at_external := bot3;
+    ModSem.at_external := bot2;
     ModSem.initial_frame := initial_frame;
     ModSem.final_frame := final_frame;
-    ModSem.after_external := bot5;
+    ModSem.after_external := bot3;
     ModSem.globalenv:= globalenv;
     ModSem.skenv := skenv;
   |}
   .
-  Next Obligation. all_prop_inv; ss. Qed.
   Next Obligation. all_prop_inv; ss. Qed.
   Next Obligation. all_prop_inv; ss. Qed.
   Next Obligation. all_prop_inv; ss. Qed.
