compose/ModSem.v
@@ -14,6 +14,32 @@ Set Implicit Arguments.
 
 
 
+Module Wenv.
+
+  Definition t: Type := block -> option signature.
+
+End Wenv.
+
+Module Args.
+
+  Record t := mk {
+    fptr: val;
+    (* sg: signature; *)
+    vs: list val;
+    m: mem;
+  }.
+
+End Args.
+
+Module Retv.
+
+  Record t := mk {
+    v: val;
+    m: mem;
+  }.
+
+End Retv.
+
 Module ModSem.
 
   (* Stores callee data that will be used only in meta-steps. *)
@@ -25,20 +51,14 @@ Module ModSem.
     step (ge: genvtype) (st0: state) (tr: trace) (st1: state): Prop;
     (* TOOD: is ge needed? I follow compcert for now. *)
 
-    get_mem (st0: state): mem;
     (* set_mem (m0: mem) (st0: state): state; *) (* This is not used, after_external is enough *)
-    at_external (st0: state)
-                (rs_arg: regset) (m_arg: mem): Prop;
-    initial_frame (rs_arg: regset) (m_arg: mem)
-                    (st0: state): Prop;
+    at_external (st0: state) (args: Args.t): Prop;
+    initial_frame (args: Args.t) (st0: state): Prop;
     (* time: rs_arg >> st0 *)
-    final_frame (rs_init: regset)
-    (* What is sg_arg/rs_arg for? Just auxiliary data. rs_arg: returning from C/ *)
-                  (st0: state)
-                  (rs_ret: regset) (* (m_ret: mem) *): Prop;
+    final_frame (* (st_init: state) *) (st0: state)
+                (retv: Retv.t): Prop;
     (* time: st0 >> rs_arg *)
-    after_external (st0: state) (rs_arg: regset)
-                   (rs_ret: regset) (m_ret: mem)
+    after_external (st0: state) (retv: Retv.t)
                    (st1: state): Prop;
     globalenv: genvtype;
     (* internals: list block; *)
@@ -59,27 +79,21 @@ Module ModSem.
     (*   , *)
     (*     <<MEM: st0.(get_mem) = m_arg>> *)
     (* ; *)
-    after_external_get_mem: forall
-        st0 rs_arg rs_ret m_ret st1
-        (AFTER: after_external st0 rs_arg rs_ret m_ret st1)
+
+    at_external_dtm: forall
+        st args0 args1
+        (AT0: at_external st args0)
+        (AT1: at_external st args1)
       ,
-        <<MEM: st1.(get_mem) = m_ret>>
+        args0 = args1
     ;
 
-    initial_frame_dtm: forall
-        rs_arg m_arg
-        st0 st1
-        (INIT0: initial_frame rs_arg m_arg st0)
-        (INIT1: initial_frame rs_arg m_arg st1)
-      ,
-        st0 = st1
-    ;
     final_frame_dtm: forall
-        rs_init st rs_ret0 rs_ret1
-        (FINAL0: final_frame rs_init st rs_ret0)
-        (FINAL1: final_frame rs_init st rs_ret1)
+        st retv0 retv1
+        (FINAL0: final_frame st retv0)
+        (FINAL1: final_frame st retv1)
       ,
-        rs_ret0 = rs_ret1
+        retv0 = retv1
     ;
     (* final_frame_dtm: forall *)
     (*     rs_init st rs_ret0 m_ret0 rs_ret1 m_ret1 *)
@@ -89,18 +103,17 @@ Module ModSem.
     (*     rs_ret0 = rs_ret1 /\ m_ret0 = m_ret1 *)
     (* ; *)
     after_external_dtm: forall
-        st_call rs_arg rs_ret m_ret st0 st1
-        (AFTER0: after_external st_call rs_arg rs_ret m_ret st0)
-        (AFTER1: after_external st_call rs_arg rs_ret m_ret st1)
+        st_call retv st0 st1
+        (AFTER0: after_external st_call retv st0)
+        (AFTER0: after_external st_call retv st1)
       ,
         st0 = st1
     ;
 
 
-    is_call (st0: state): Prop := exists rs_arg m_arg, at_external st0 rs_arg m_arg;
+    is_call (st0: state): Prop := exists args, at_external st0 args;
     is_step (st0: state): Prop := exists tr st1, step globalenv st0 tr st1;
-    is_return (rs_init: regset) (st0: state): Prop := exists rs_ret, final_frame rs_init st0 rs_ret;
-    may_return (st0: state): Prop := exists rs_init, is_return rs_init st0;
+    is_return (st0: state): Prop := exists retv, final_frame st0 retv;
       (* exists rs_init rs_ret m_ret, final_frame rs_init st0 rs_ret m_ret; *)
     (* Note: "forall" or "exists" for rs_init? *)
     (* "forall" -> easy for opt/hard for meta *)
@@ -109,8 +122,8 @@ Module ModSem.
     (* We can think of something like "forall rs_init (FUTURE: st0 is future of rs_init)", but is overkill. *)
 
     call_step_disjoint: is_call /1\ is_step <1= bot1;
-    step_return_disjoint: is_step /1\ may_return <1= bot1;
-    call_return_disjoint: is_call /1\ may_return <1= bot1;
+    step_return_disjoint: is_step /1\ is_return <1= bot1;
+    call_return_disjoint: is_call /1\ is_return <1= bot1;
 
     (* step_at_external_disjoint: forall *)
     (*     st0 *)
@@ -173,7 +186,7 @@ Module ModSem.
 
 End ModSem.
 
-Hint Unfold ModSem.is_call ModSem.is_step ModSem.may_return ModSem.is_return ModSem.get_mem.
+Hint Unfold ModSem.is_call ModSem.is_step ModSem.is_return.
 
 Coercion ModSem.to_semantics: ModSem.t >-> semantics.
 (* I want to use definitions like "Star" or "determinate_at" *)
