compose/SimSymb.v
@@ -12,313 +12,12 @@ Require Import ASTC.
 Require Import LinkingC.
 Require Import Maps.
 
-Require Import SimDef SimMem.
+Require Import SimMem.
 
 Set Implicit Arguments.
 
 
 Module SimSymb.
-
-  (* I wanted to use "t" as ss0/ss_linked, but forward reference is impossible. *)
-  Inductive link_exact_preserved (ss0: ident -> ident -> Prop) (sk_src: Sk.t) (sk_tgt: Sk.t) (ss_linked: ident -> ident -> Prop): Prop :=
-  | link_exact_preserved_intro
-      (EXACT: forall
-          id_src id_tgt
-          (SRCIN: sk_src.(privs_old) id_src)
-          (TGTIN: sk_tgt.(privs_old) id_tgt)
-        ,
-          <<EXACT: ss0 id_src id_tgt <-> ss_linked id_src id_tgt>>)
-  .
-
-  Definition injective_func X Y (inj: X -> option Y): Prop := forall
-      x0 x1 y
-      (INJ0: inj x0 = Some y)
-      (INJ1: inj x1 = Some y)
-    ,
-      x0 = x1
-  .
-
-  (* TODO: better name *)
-  Inductive injective_rel X Y (inj: X -> Y -> Prop): Prop :=
-  | injective_domain
-      (DOMAIN: forall
-          x0 x1 y
-          (INJ0: inj x0 y)
-          (INJ1: inj x1 y)
-        ,
-          x0 = x1)
-  | injective_image
-      (IMAGE: forall
-          x y0 y1
-          (INJ0: inj x y0)
-          (INJ1: inj x y1)
-        ,
-          y0 = y1)
-  .
-
-  Inductive wf' (sim_symb: ident -> ident -> Prop) (privs_old: ident -> Prop) :=
-  | wf_intro
-      (CLOSED: forall
-          id_src id_tgt
-          (SIM: sim_symb id_src id_tgt)
-        ,
-          <<SRC: privs_old id_src>> /\ <<TGT: privs_old id_tgt>>)
-      (INJ: injective_rel sim_symb)
-  .
-
-
-
-  (* Properties that are needed in meta-theory. *)
-Module DEPRECATED.
-  Inductive sim_sk_weak (coverage kept: ident -> Prop) (sk_src sk_tgt: Sk.t): Prop :=
-  | sim_sk_weak_intro
-      (WF: (kept <1= coverage))
-      (* We can pull "WF" out, it dosen't require sk_src/sk_tgt. But is it meaningful? *)
-      (INSRC: (coverage <1= sk_src.(privs_old)))
-      (INTGT: (coverage <1= sk_tgt.(privs_old)))
-      (* Is both are needed? *)
-      (NOCOVER: forall
-          id
-          (PUBS: ~ coverage id)
-        ,
-          <<SIM: sim_odef (sk_src.(prog_defmap) ! id) (sk_tgt.(prog_defmap) ! id)>>)
-      (* Further, we can say equality instead of sim, for public defs. Is it needed? *)
-      (KEPT: forall
-          id
-          (* (COVER: coverage id) *)
-          (KEPT: kept id)
-        ,
-          <<SIM: sim_odef (sk_src.(prog_defmap) ! id) (sk_tgt.(prog_defmap) ! id)>>)
-      (NOKEPT: forall
-          id
-          (COVER: coverage id)
-          (NOKEPT: ~ kept id)
-        ,
-          <<NOKEPT: None = sk_tgt.(prog_defmap) ! id>>)
-      (MAINKEPT: <<KEPT: kept sk_src.(prog_main)>> \/ <<NOCOVER: ~ coverage sk_src.(prog_main)>>)
-      (* TODO: Remove PUB/MAIN from SimModPair *)
-      (PUB: sk_src.(prog_public) = sk_tgt.(prog_public))
-      (MAIN: sk_src.(prog_main) = sk_tgt.(prog_main))
-  .
-
-  Lemma sim_sk_weak_def_bsim
-        coverage kept sk_src sk_tgt
-        (CLOSED: sim_sk_weak coverage kept sk_src sk_tgt)
-        id def_tgt
-        (DEFTGT: sk_tgt.(prog_defmap) ! id = Some def_tgt)
-    :
-      exists def_src, <<DEFSRC: sk_src.(prog_defmap) ! id = Some def_src>> /\ <<SIM: sim_def def_src def_tgt>>
-  .
-  Proof.
-    inv CLOSED.
-    destruct (classic (coverage id)).
-    - destruct (classic (kept id)).
-      + exploit KEPT; eauto. intro SIM.
-        inv SIM.
-        { eq_closure_tac. esplits; eauto. }
-        exfalso. congruence.
-      + exploit NOKEPT; eauto. i. congruence.
-    - exploit NOCOVER; eauto. intro SIM.
-      inv SIM.
-      { eq_closure_tac. esplits; eauto. }
-      exfalso. congruence.
-  Qed.
-
-  Lemma sim_sk_weak_enables_link
-        (sk_src0 sk_tgt0: Sk.t)
-        kept0 coverage0
-        (CLOSED0: sim_sk_weak coverage0 kept0 sk_src0 sk_tgt0)
-        sk_src1 sk_tgt1
-        kept1 coverage1
-        (CLOSED1: sim_sk_weak coverage1 kept1 sk_src1 sk_tgt1)
-        sk_src
-        (LINKSRC: link sk_src0 sk_src1 = Some sk_src)
-    :
-      exists sk_tgt, <<LINKTGT: link sk_tgt0 sk_tgt1 = Some sk_tgt>>
-  .
-  Proof.
-    Local Transparent Linker_prog. ss. Local Opaque Linker_prog.
-    exploit (link_prog_inv sk_src0 sk_src1); eauto. intro LINKSPEC; des. inv LINKSPEC. des.
-    exploit (link_prog_succeeds sk_tgt0 sk_tgt1); eauto.
-    - inv CLOSED0. inv CLOSED1. ss.
-      eq_closure_tac.
-    - i.
-      exploit sim_sk_weak_def_bsim; try apply H; eauto. i; des.
-      exploit sim_sk_weak_def_bsim; try apply H0; eauto. i; des.
-      exploit BOTHHIT; eauto. i; des.
-      inv CLOSED0. inv CLOSED1. ss.
-      esplits; eauto.
-      + rewrite <- PUB; ss.
-      + rewrite <- PUB0; ss.
-      + exploit sim_def_preserves_link; eauto. i; des_safe. ii. clarify.
-  Qed.
-
-End DEPRECATED.
-
-  Inductive sim_sk_weak (coverage: ident -> Prop) (sk_src sk_tgt: Sk.t): Prop :=
-  | sim_sk_weak_intro
-      (* (INSRC: (coverage <1= sk_src.(privs_old))) *)
-      (COVERAGE: (coverage <1= sk_tgt.(privs_old)))
-      (PRIVS_OLD: sk_tgt.(privs_old) <1= sk_src.(privs_old))
-      (NOCOVER: forall
-          id
-          (PUBS: ~ coverage id)
-        ,
-          <<SIM: sim_odef (sk_src.(prog_defmap) ! id) (sk_tgt.(prog_defmap) ! id)>>)
-      (COVER: forall
-          id
-          (COVER: coverage id)
-          def_tgt
-          (DEFTGT: sk_tgt.(prog_defmap) ! id = Some def_tgt)
-        ,
-          exists def_src, <<DEFSRC: sk_src.(prog_defmap) ! id = Some def_src>>)
-      (PUB: sk_src.(prog_public) = sk_tgt.(prog_public))
-      (MAIN: sk_src.(prog_main) = sk_tgt.(prog_main))
-  .
-
-  Lemma sim_sk_weak_def_bsim
-        coverage sk_src sk_tgt
-        (CLOSED: sim_sk_weak coverage sk_src sk_tgt)
-        id def_tgt
-        (DEFTGT: sk_tgt.(prog_defmap) ! id = Some def_tgt)
-    :
-      exists def_src, <<DEFSRC: sk_src.(prog_defmap) ! id = Some def_src>>
-                     /\ <<SIM: ~(coverage id) -> sim_def def_src def_tgt>>
-  .
-  Proof.
-    inv CLOSED.
-    destruct (classic (coverage id)).
-    - exploit COVER; eauto. i; des.
-      esplits; eauto. ii. ss.
-    - exploit NOCOVER; eauto. intro SIM.
-      inv SIM.
-      { eq_closure_tac. esplits; eauto. }
-      exfalso. congruence.
-  Qed.
-
-  Lemma sim_sk_weak_enables_link
-        (sk_src0 sk_tgt0: Sk.t)
-        coverage0
-        (CLOSED0: sim_sk_weak coverage0 sk_src0 sk_tgt0)
-        sk_src1 sk_tgt1
-        coverage1
-        (CLOSED1: sim_sk_weak coverage1 sk_src1 sk_tgt1)
-        sk_src
-        (LINKSRC: link sk_src0 sk_src1 = Some sk_src)
-    :
-      exists sk_tgt, <<LINKTGT: link sk_tgt0 sk_tgt1 = Some sk_tgt>>
-  .
-  Proof.
-    Local Transparent Linker_prog. ss. Local Opaque Linker_prog.
-    exploit (link_prog_inv sk_src0 sk_src1); eauto. intro LINKSPEC; des. inv LINKSPEC. des.
-    exploit (link_prog_succeeds sk_tgt0 sk_tgt1); eauto.
-    - inv CLOSED0. inv CLOSED1. ss.
-      eq_closure_tac.
-    - i.
-      exploit sim_sk_weak_def_bsim; try apply H; eauto. i; des.
-      exploit sim_sk_weak_def_bsim; try apply H0; eauto. i; des.
-      exploit BOTHHIT; eauto. i; des.
-      inv CLOSED0. inv CLOSED1. ss.
-      exploit SIM. { intro T. eapply COVERAGE in T. inv T; des. eapply H5. rewrite <- PUB; ss. } i; des.
-      exploit SIM0. { intro T. eapply COVERAGE0 in T. inv T; des. eapply H6. rewrite <- PUB0; ss. } i; des.
-      esplits; eauto.
-      + rewrite <- PUB; ss.
-      + rewrite <- PUB0; ss.
-      + exploit sim_def_preserves_link; eauto. i; des_safe. ii. clarify.
-  Qed.
-
-
-  (* Inductive load_exact_preserved `{SS: SimSymb.SimSymb} `{SM: SimMem.SimMem} *)
-  (*           (ss0: SimSymb.t) (sk_src sk_tgt: Sk.t) *)
-  (*           (sm0: SimMem.t) (skenv_src skenv_tgt: SkEnv.t): Prop := *)
-  (* | exact_preserved_intro *)
-  (*     (COMPAT: forall *)
-  (*         id_src id_tgt b_src b_tgt *)
-  (*         (SRCB: skenv_src.(Genv.find_symbol) id_src = Some b_src) *)
-  (*         (TGTB: skenv_tgt.(Genv.find_symbol) id_tgt = Some b_tgt) *)
-  (*       , *)
-  (*         sm0.(SimMem.sim_val) (Vptr b_src Ptrofs.zero true) (Vptr b_tgt Ptrofs.zero true) <-> *)
-  (*         ss0.(SimSymb.sim_symb) id_src id_tgt) *)
-  (* . *)
-
-  (* Inductive sim_skenv *)
-  (*           (kept: ident -> Prop) (sm: SimMem.t) *)
-  (*           (skenv_src skenv_tgt: SkEnv.t): Prop := *)
-  (* | sim_skenv_intro *)
-  (*     (SIMSYMB1: forall *)
-  (*         id blk_src blk_tgt delta *)
-  (*         (SIMVAL: SimMem.sim_val sm (Vptr blk_src Ptrofs.zero true) (Vptr blk_tgt Ptrofs.zero true)) *)
-  (*         (BLKSRC: skenv_src.(Genv.find_symbol) id = Some blk_src) *)
-  (*       , *)
-  (*         <<DELTA: delta = 0>> /\ <<BLKTGT: skenv_tgt.(Genv.find_symbol) id = Some blk_tgt>>) *)
-  (*     (SIMSYMB2: forall *)
-  (*         id *)
-  (*         (KEPT: kept id) *)
-  (*         blk_src *)
-  (*         (BLKSRC: skenv_src.(Genv.find_symbol) id = Some blk_src) *)
-  (*       , *)
-  (*         exists blk_tgt, *)
-  (*           <<BLKTGT: skenv_tgt.(Genv.find_symbol) id = Some blk_tgt>> /\ *)
-  (*           <<SIM: SimMem.sim_val sm (Vptr blk_src Ptrofs.zero true) (Vptr blk_tgt Ptrofs.zero true)>>) *)
-  (*     (SIMSYMB3: forall *)
-  (*         id blk_tgt *)
-  (*         (BLKTGT: skenv_tgt.(Genv.find_symbol) id = Some blk_tgt) *)
-  (*       , *)
-  (*         exists blk_src, *)
-  (*           <<BLKSRC: skenv_src.(Genv.find_symbol) id = Some blk_src>> /\ *)
-  (*           <<SIM: SimMem.sim_val sm (Vptr blk_src Ptrofs.zero true) (Vptr blk_tgt Ptrofs.zero true)>>) *)
-  (* . *)
-
-  (* Inductive sim_skenv_spec (coverage kept: ident -> Prop) (skenv_src skenv_tgt: SkEnv.t): Prop := *)
-  (* | sim_skenv_spec_intro *)
-  (*     (SPEC: forall *)
-  (*         id *)
-  (*         (KEPT: kept id) *)
-  (*       , *)
-  (*         skenv_src.(Genv.find_symbol) id = skenv_src.(Genv.find_symbol) id) *)
-  (* . *)
-
-  Inductive sk_def_bsim (sk_src sk_tgt: Sk.t): Prop :=
-  | sk_def_bsim_intro
-      (DEFBSIM: forall
-          id def_tgt
-          (DEFTGT: sk_tgt.(prog_defmap) ! id = Some def_tgt)
-        ,
-          exists def_src, <<DEFSRC: sk_src.(prog_defmap) ! id = Some def_src>> /\
-                                    <<SIM: sim_def def_src def_tgt>>)
-  .
-
-
-(* I think this is the minimal spec required for lock-step modsem finding *)
-  Inductive skenv_func_bsim `{SimMem.class} (sm0: SimMem.t) (skenv_src skenv_tgt: SkEnv.t): Prop :=
-  | skenv_def_bsim_intro
-      (FUNCBSIM: forall
-          fptr_src fptr_tgt def_tgt
-          (SIMFPTR: sm0.(SimMem.sim_val) fptr_src fptr_tgt)
-          (FUNCTGT: skenv_tgt.(Genv.find_funct) fptr_tgt = Some def_tgt)
-          (SAFESRC: exists _def_src, skenv_src.(Genv.find_funct) fptr_src = Some _def_src)
-        ,
-          exists def_src, <<FUNCSRC: skenv_src.(Genv.find_funct) fptr_src = Some def_src>> /\
-                          <<SIM: sim_fun def_src def_tgt>>)
-      (FUNCPROGRESS: forall
-          fptr_src fptr_tgt
-          (SIMFPTR: sm0.(SimMem.sim_val) fptr_src fptr_tgt)
-          (SAFESRC: exists _def_src, skenv_src.(Genv.find_funct) fptr_src = Some _def_src)
-        ,
-          exists def_tgt, <<PROGRESS: skenv_tgt.(Genv.find_funct) fptr_tgt = Some def_tgt>>)
-  .
-
-(* These statements are direct copy from Unusedglobproof.v - defs_inject, EXCEPT for ref_def *)
-  Inductive skenv_func_fsim `{SimMem.class} (sm0: SimMem.t) (skenv_src skenv_tgt: SkEnv.t): Prop :=
-  | skenv_def_fsim_intro
-      (FUNCSIM: forall
-          fptr_src fptr_tgt def_src
-          (SIMFPTR: sm0.(SimMem.sim_val) fptr_src fptr_tgt)
-          (FUNCSRC: skenv_src.(Genv.find_funct) fptr_src = Some def_src)
-        ,
-          exists def_tgt, <<FUNCSRC: skenv_tgt.(Genv.find_funct) fptr_tgt = Some def_tgt>> /\
-                          <<SIM: sim_fun def_src def_tgt>>)
-  .
 
   Inductive skenv_func_bisim (sim_val: val -> val -> Prop) (skenv_src skenv_tgt: SkEnv.t): Prop :=
   | skenv_func_bisim_intro
@@ -328,7 +27,7 @@ End DEPRECATED.
           (FUNCSRC: skenv_src.(Genv.find_funct) fptr_src = Some def_src)
         ,
           exists def_tgt, <<FUNCSRC: skenv_tgt.(Genv.find_funct) fptr_tgt = Some def_tgt>> /\
-                          <<SIM: sim_fun def_src def_tgt>>)
+                          <<SIM: def_src = def_tgt>>)
       (FUNCBSIM: forall
           fptr_src fptr_tgt def_tgt
           (SAFESRC: is_real_ptr fptr_src)
@@ -336,7 +35,7 @@ End DEPRECATED.
           (FUNCTGT: skenv_tgt.(Genv.find_funct) fptr_tgt = Some def_tgt)
         ,
           exists def_src, <<FUNCSRC: skenv_src.(Genv.find_funct) fptr_src = Some def_src>> /\
-                          <<SIM: sim_fun def_src def_tgt>>)
+                          <<SIM: def_src = def_tgt>>)
   .
 
   (* TODO: Try moving t into argument? sim_symb coercion gets broken and I don't know how to fix it. *)
@@ -361,13 +60,7 @@ End DEPRECATED.
       ;
 
       sim_sk: t -> Sk.t -> Sk.t -> Prop;
-      (* Do we need this ? *)
-      (* sim_sk_def_bsim: forall *)
-      (*     ss sk_src sk_tgt *)
-      (*     (SIMSK: sim_sk ss sk_src sk_tgt) *)
-      (*   , *)
-      (*     <<DEF: sk_def_bsim sk_src sk_tgt>> *)
-      (* ; *)
+
       sim_sk_link: forall
           ss0 (sk_src0 sk_tgt0: Sk.t)
           (SIMSK: sim_sk ss0 sk_src0 sk_tgt0)
@@ -466,26 +159,6 @@ End DEPRECATED.
           <<SIMSKENV: sim_skenv sm ss skenv_src skenv_tgt>>
       ;
 
-      (* sim_skenv_def_bsim: forall *)
-      (*     sm ss skenv_src skenv_tgt *)
-      (*     (SIMSKENV: sim_skenv sm ss skenv_src skenv_tgt) *)
-      (*   , *)
-      (*     <<DEF: skenv_def_bsim sm skenv_src skenv_tgt>> *)
-      (* ; *)
-
-
-      (* sim_skenv_func_fsim: forall *)
-      (*     sm ss skenv_src skenv_tgt *)
-      (*     (SIMSKENV: sim_skenv sm ss skenv_src skenv_tgt) *)
-      (*   , *)
-      (*     <<DEF: skenv_func_fsim sm skenv_src skenv_tgt>> *)
-      (* ; *)
-      (* sim_skenv_func_bsim: forall *)
-      (*     sm ss skenv_src skenv_tgt *)
-      (*     (SIMSKENV: sim_skenv sm ss skenv_src skenv_tgt) *)
-      (*   , *)
-      (*     <<DEF: skenv_func_bsim sm skenv_src skenv_tgt>> *)
-      (* ; *)
       sim_skenv_func_bisim: forall
           sm ss skenv_src skenv_tgt
           (SIMSKENV: sim_skenv sm ss skenv_src skenv_tgt)
@@ -495,71 +168,5 @@ End DEPRECATED.
     }
   .
 
-  (* Module TMP. *)
-  (*   Section TMP. *)
-  (*   Context `{SS: class}. *)
-  (*   Axiom ss0: t. *)
-  (*   Axiom i: ident. *)
-  (*   Fail Check (ss0 i). *)
-  (*   Coercion sim_symb: t >-> Funclass. *)
-  (*   Check (ss0 i). *)
-  (*   End TMP. *)
-  (* End TMP. *)
-
-
 End SimSymb.
-
-(* Coercion SimSymb.sim_symb: SimSymb.t >-> Funclass. *)
-
-(* Module TMP. *)
-(*   Variable T: Type. *)
-(*   Context `{SS: SimSymb.class T}. *)
-(*   Axiom ss0: T. *)
-(*   Axiom i: ident. *)
-(*   Check (SimSymb.sim_symb ss0 i). *)
-(*   Fail Check (ss0 i). *)
-(*   Coercion SimSymb.sim_symb: SimSymb.class >-> Funclass. *)
-(*   Fail Check (ss0 i). *)
-(* End TMP. *)
-
-
-(* Print Coercions. *)
-
-(* Variables X: Type. *)
-(* Context `{SimSymb X}. *)
-(* Variable x: X. *)
-(* Variable i0: ident. *)
-(* Fail Check (x i0). *)
-(* Check (sim_symb x i0). *)
-(* (* Coercion sim_symb: SimSymb >-> Funclass. *) *)
-(* (* Fail Check (x i0). *) *)
-(* Coercion sim_symb: X >-> Funclass. *)
-(* Print Coercions. *)
-(* Coercion sim_symb: forall (X: Type) `{SimSymb X}, X >-> Funclass. *)
-
-
-(* TODO: name? *)
-(* Inductive closed `{SimSymb.class} (ss: SimSymb.t) (sk_src sk_tgt: Sk.t): Prop := *)
-(* | closed_intro *)
-(*     (WF: SimSymb.wf ss) *)
-(*     (INSRC: all1 (ss.(SimSymb.coverage) <1= sk_src.(privs_old))) *)
-(*     (INTGT: all1 (ss.(SimSymb.coverage) <1= sk_tgt.(privs_old))) *)
-(*     (NOCOVER: forall *)
-(*         id *)
-(*         (PUBS: ~ ss.(SimSymb.coverage) id) *)
-(*       , *)
-(*         <<EQ: sk_src.(prog_defmap) ! id = sk_tgt.(prog_defmap) ! id>>) *)
-(*     (KEPT: forall *)
-(*         id *)
-(*         (COVER: ss.(SimSymb.coverage) id) *)
-(*         (KEPT: ss.(SimSymb.kept) id) *)
-(*       , *)
-(*         <<EQ: sk_src.(prog_defmap) ! id = sk_tgt.(prog_defmap) ! id>>) *)
-(*     (NOKEPT: forall *)
-(*         id *)
-(*         (COVER: ss.(SimSymb.coverage) id) *)
-(*         (NOKEPT: ~ ss.(SimSymb.kept) id) *)
-(*       , *)
-(*         <<NOKEPT: None = sk_tgt.(prog_defmap) ! id>>) *)
-(* . *)
 
